Updated lab classes Added missing files from previous handouts, also added new lab classes developed with VeryFast

Aula6/Lab6/Bank.java
@@ -1,0 +1,87 @@
+/*
+Starting point for exercise of Lab Session 6.
+CVS course - Integrated Master in Computer Science and Engineering
+@FCT UNL Luis Caires 2015
+*/
+
+/*@
+predicate AccountP(unit a,BankAccount c; int n) = c != null &*& AccountInv(c,n,?m);
+@*/
+
+/*@
+predicate BankInv(Bank bk; int n, int m) = 
+     bk.nelems |-> n &*& 
+     bk.capacity |-> m &*& 
+     m > 0 &*&
+     bk.store |-> ?a &*&
+     a != null &*&
+     a.length == m &*&
+     0 <= n &*& n<=m &*& 
+     array_slice_deep(a, 0, n, AccountP, unit,_,?bs) &*&
+     array_slice(a, n, m,?rest) &*& 
+     all_eq(rest, null) == true ;
+@*/
+
+
+class Bank {
+
+  BankAccount store[];
+  int nelems;
+  int capacity;
+
+  public Bank(int size)
+  //@ requires 0 < size;
+  //@ ensures BankInv(this,0,size);
+  {
+    nelems = 0;
+    capacity = siz;
+    store = new BankAccount[siz];
+  }
+
+  void addnewAccount(int code)
+     //@ requires BankInv(this,?n, ?m) &*& code >= 0;
+     //@ ensures BankInv(this,n+1,m);
+  
+  {
+   	BankAccount c = new BankAccount(code);
+  	store[nelems] = c;
+    nelems = nelems + 1;
+  }
+
+  int getbalance(int code)
+     //@ requires BankInv(this,?n, ?m);
+     //@ ensures BankInv(this,n+1,m);
+  
+  {
+    int i = 0;
+
+    while (i < nelems)
+    //@ invariant BankInv(this,n,m) &*& 0 <= i &*& i <= n;
+    {
+       if ( store[i].getcode() == code) {
+       	return store[i].getbalance();
+       }
+       i = i + 1;
+    }
+    return -1;
+  }
+
+  int removeAccount(int code)
+  {
+    int i = 0;
+    while (i < nelems)
+    //@ invariant BankInv(this,n,m) &*& 0 <= i &*& i <= n;
+    {
+       if ( store[i].getcode() == code) {
+       	   if (i<nelems-1) {
+       	     store[i] == store[nelems-1];
+       	   }
+       	   nelems = nelems - 1;
+       	   store[nelems] = null;
+       	 return 0;
+       }
+       i = i + 1;
+    }
+    return -1;
+  }
+}
