Aula6/Lab6/BankAccount.java
@@ -1,0 +1,56 @@
+/*
+Starting point for exercise of Lab Session 6.
+CVS course - Integrated Master in Computer Science and Engineering
+@FCT UNL 2018
+*/
+
+
+public class BankAccount {
+
+  int balance;
+  int climit;
+  int accountid;
+
+  public BankAccount(int id)
+  {
+      balance = 0;
+      climit = 0;
+      accountid = id;
+  }
+
+  public void deposit(int v)
+  {
+  balance += v;
+  }
+
+  public void withdraw(int v)
+  {
+     balance  -= v;
+  }
+
+  public int getcode()
+  {
+     return accountid;
+  }
+
+  public int getbalance()
+  {
+     return balance;
+  }
+
+  public void setclimit(int cl)
+  {
+      climit = cl;
+  }
+
+  public int getclimit()
+  {
+     return climit;
+  }
+
+  static void main()
+  {
+    BankAccount b1 = new BankAccount(1000);
+    b1.setclimit(500);
+  }
+}
