Aula7/CCCounter.java
@@ -1,0 +1,157 @@
+import java.util.concurrent.*;
+import java.util.concurrent.locks.*;
+
+/*@
+
+predicate_ctor BCounter_shared_state (BCounter c) () =
+   c.N |-> ?v &*& v >= 0 &*& c.MAX |-> ?m &*& m > 0 &*& v <= m;
+
+predicate_ctor BCounter_nonzero (BCounter c) () =
+   c.N |-> ?v &*& c.MAX |-> ?m &*& v > 0 &*& m > 0 &*& v <= m; 
+
+predicate_ctor BCounter_nonmax (BCounter c) () =
+   c.N |-> ?v &*& c.MAX |-> ?m &*& v < m &*& m > 0 &*& v >= 0; 
+
+predicate BCounterInv(BCounter c) = 
+        c.mon |-> ?l 
+    &*& l != null 
+    &*& lck(l,1, BCounter_shared_state(c)) 
+    &*& c.notzero |-> ?cc 
+    &*& cc !=null 
+    &*& cond(cc, BCounter_shared_state(c), BCounter_nonzero(c))
+    &*& c.notmax |-> ?cm 
+    &*& cm !=null 
+    &*& cond(cm, BCounter_shared_state(c), BCounter_nonmax(c));
+@*/
+
+
+class BCounter {
+  int N;
+  int MAX;
+  ReentrantLock mon;
+  Condition notzero;
+  Condition notmax;
+
+  BCounter(int max)
+  //@ requires 0 < max;
+  //@ ensures BCounterInv(this);
+  { 
+      N = 0 ; 
+      MAX = max; 
+      //@ close BCounter_shared_state(this)();
+      //@ close enter_lck(1,BCounter_shared_state(this));
+      mon = new ReentrantLock(); 
+      //@ close set_cond(BCounter_shared_state(this),BCounter_nonzero(this));
+      notzero = mon.newCondition();
+      //@ close set_cond(BCounter_shared_state(this),BCounter_nonmax(this));
+      notmax = mon.newCondition();
+      //@ close BCounterInv(this);
+  }
+
+  void inc()
+  //@ requires BCounterInv(this);
+  //@ ensures BCounterInv(this);
+  { 
+      //@ open BCounterInv(this);
+      // request permission to enter the monitor and access 
+      // the conditions and the values of the fields N and MAX.
+      mon.lock();
+      //@ open BCounter_shared_state(this)();
+      // Wait for the preconditions of the operations to hold.
+      // Wait until the condition is met or another thread releases 
+      // the monitor in a compatible state.
+      
+  
+	//if( N == MAX ){
+	//	//@ close BCounter_shared_state(this)();
+	//	notmax.wait();
+	//	//@ open BCounter_nonmax(this)();
+	//}
+      
+     // But we need a loop to avoid spurious wakeps
+      while ( N == MAX ) 
+      /*@ invariant this.N |-> ?v 
+      	          &*& v >= 0 
+      	          &*& this.MAX |-> ?m 
+      	          &*& m > 0 
+      	          &*& v <= m 
+      	          &*& this.notzero |-> ?cc 
+      	          &*& cc !=null 
+      	          &*& cond(cc, BCounter_shared_state(this), BCounter_nonzero(this)) 
+      	          &*& this.notmax |-> ?cm
+      	          &*& cm !=null 
+      	          &*& cond(cm, BCounter_shared_state(this), BCounter_nonmax(this));
+      @*/
+      { // The invariant is necessary to propagate the knowledge
+        //@ close BCounter_shared_state(this)(); 
+	notmax.await();
+      	//@ open BCounter_nonmax(this)(); 
+      }
+
+      N++;
+      //@ close BCounter_nonzero(this)();
+      notzero.signal();
+      mon.unlock(); // release ownership of the shared state
+      //@ close BCounterInv(this);
+  } 
+
+  void dec()
+  //@ requires BCounterInv(this);
+  //@ ensures BCounterInv(this);
+  { 
+      //@ open BCounterInv(this);
+      mon.lock(); // request permission to the shared state
+      //@ open BCounter_shared_state(this)();
+      while ( N == 0 )
+      	/*@ invariant this.N |-> ?v 
+      	          &*& v >= 0 
+      	          &*& this.MAX |-> ?m 
+      	          &*& m > 0 
+      	          &*& v <= m 
+      	          &*& this.notzero |-> ?cc 
+      	          &*& cc !=null 
+      	          &*& cond(cc, BCounter_shared_state(this), BCounter_nonzero(this)) 
+      	          &*& this.notmax |-> ?cm
+      	          &*& cm !=null 
+      	          &*& cond(cm, BCounter_shared_state(this), BCounter_nonmax(this)); 
+      	@*/
+      {
+        //@ close BCounter_shared_state(this)(); 
+      	notzero.await();
+      	//@ open BCounter_nonzero(this)(); 
+      }
+      //@ assert N > 0;
+
+      N--; 
+      //@ assert N < MAX;
+      //@ close BCounter_nonmax(this)(); 
+      notmax.signal();
+      mon.unlock(); // release ownership of the shared state
+      //@ close BCounterInv(this);
+  } 
+  
+  int get()
+  //@ requires BCounterInv(this);
+  //@ ensures BCounterInv(this);
+  { 
+      int r;
+      //@ open BCounterInv(this);
+      mon.lock(); 
+      //@ open BCounter_shared_state(this)();
+      r = N; // put a copy on the stack, private to the thread
+      //@ close BCounter_shared_state(this)();
+      mon.unlock();	
+      //@ close BCounterInv(this);
+      return r;
+  } 
+
+  public static void main(String[] args) 
+  //@ requires true;
+  //@ ensures true;
+  {
+       int MAX = 100;
+       BCounter c = new BCounter(MAX);
+       //@ assert BCounterInv(c);
+       c.inc();         
+  }
+}
