Aula7/CCounter.java
@@ -1,0 +1,81 @@
+import java.util.concurrent.*;
+import java.util.concurrent.locks.*;
+
+/*@ 
+    predicate_ctor BCounter_shared_state (BCounter c) () =
+        c.N |-> ?v &*& v >= 0 &*& c.MAX |-> ?m &*& m > 0 &*& v <= m;
+@*/
+
+/*@ predicate BCounterInv(BCounter c) = 
+    c.mon |-> ?l &*&
+    l != null &*& lck(l,1,BCounter_shared_state(c));
+@*/
+
+class BCounter {
+  int N;
+  int MAX;
+  ReentrantLock mon;
+
+  BCounter(int max)
+  //@ requires 0 < max;
+  //@ ensures BCounterInv(this);
+  { 
+      N = 0 ; 
+      MAX = max; 
+      //@ close BCounter_shared_state(this)();
+      //@ close enter_lck(1,BCounter_shared_state(this));
+      mon = new ReentrantLock(); 
+      //@ close BCounterInv(this);
+  }
+
+  void inc()
+  //@ requires BCounterInv(this);
+  //@ ensures BCounterInv(this);
+  { 
+      //@ open BCounterInv(this);
+      mon.lock(); // request permission to the shared state
+      //@ open BCounter_shared_state(this)();
+      if ( N < MAX ) N++;
+      //@ close BCounter_shared_state(this)();
+      mon.unlock(); // release ownership of the shared state
+      //@ close BCounterInv(this);
+  } 
+
+  void dec()
+  //@ requires BCounterInv(this);
+  //@ ensures BCounterInv(this);
+  { 
+      //@ open BCounterInv(this);
+      mon.lock(); // request permission to the shared state
+      //@ open BCounter_shared_state(this)();
+      if ( N > 0 ) N--; 
+      //@ close BCounter_shared_state(this)();
+      mon.unlock(); // release ownership of the shared state
+      //@ close BCounterInv(this);
+  } 
+  
+  int get()
+  //@ requires BCounterInv(this);
+  //@ ensures BCounterInv(this);
+  { 
+      int r;
+      //@ open BCounterInv(this);
+      mon.lock(); 
+      //@ open BCounter_shared_state(this)();
+      r = N; // put a copy on the stack, private to the thread
+      //@ close BCounter_shared_state(this)();
+      mon.unlock();	
+      //@ close BCounterInv(this);
+      return r;
+  } 
+
+  public static void main(String[] args) 
+  //@ requires true;
+  //@ ensures true;
+  {
+       int MAX = 100;
+       BCounter c = new BCounter(MAX);
+       //@ assert BCounterInv(c);
+       c.inc();         
+  }
+}
