Aula7/Queue.java
@@ -1,0 +1,144 @@
+import java.util.concurrent.*;
+import java.util.concurrent.locks.*;
+
+/*
+predicate_ctor BCounter_shared_state (BCounter c) () =
+   c.N |-> ?v &*& v >= 0 &*& c.MAX |-> ?m &*& m > 0 &*& v <= m;
+
+predicate_ctor BCounter_nonzero (BCounter c) () =
+   c.N |-> ?v &*& c.MAX |-> ?m &*& v > 0 &*& m > 0 &*& v <= m; 
+
+predicate_ctor BCounter_nonmax (BCounter c) () =
+   c.N |-> ?v &*& c.MAX |-> ?m &*& v < m &*& m > 0 &*& v >= 0; 
+
+predicate BCounterInv(BCounter c) = 
+        c.mon |-> ?l 
+    &*& l != null 
+    &*& lck(l,1, BCounter_shared_state(c)) 
+    &*& c.notzero |-> ?cc 
+    &*& cc !=null 
+    &*& cond(cc, BCounter_shared_state(c), BCounter_nonzero(c))
+    &*& c.notmax |-> ?cm 
+    &*& cm !=null 
+    &*& cond(cm, BCounter_shared_state(c), BCounter_nonmax(c));
+    
+
+*/
+
+
+/*@   
+predicate Queue(Queue q) = 
+	0 < a.Length &&
+        0 <= front < a.Length &&
+        0 <= rear < a.Length &&
+        if front == rear then
+            numberOfElements == 0 ||
+            numberOfElements == a.Length
+        else    
+            numberOfElements == if front > rear then front - rear
+                                                else front - rear + a.Length
+@*/
+
+
+
+class Queue {
+    
+    // Representation type
+    
+    int[] a;
+    int front;
+    int rear;
+    
+    int numberOfElements;
+    
+    Queue()
+    {
+	front = end = numberOfElements = 0;
+    	a[] = new int[numberOfElements];
+
+    }
+
+    public boolean RepInv()
+    {
+    	0 < a.Length &&
+        0 <= front < a.Length &&
+        0 <= rear < a.Length &&
+        if front == rear then
+            numberOfElements == 0 ||
+            numberOfElements == a.Length
+        else    
+            numberOfElements == if front > rear then front - rear
+                                                else front - rear + a.Length
+    
+    }
+    
+    
+    //predicados
+    public boolean NotEmpty()
+    {
+	return RepInv() && numberOfElements > 0;
+    
+    }
+
+    public boolean NotFull()
+    {
+    	return RepInv() && numberOfElements < a.Length;
+    }
+   
+   
+    public boolean Full()
+    {
+    	return numberOfElements == a.Length;
+    }
+
+   
+    public boolean Empty()
+    {
+	return numberOfElements == 0;    
+    }   
+   
+   //predicados end
+
+  
+    public void Enqueue(int V)
+    {
+    	a[front] = V;
+        front = (front + 1)%a.Length;    
+        numberOfElements = numberOfElements + 1;
+    }
+  
+    public void Dequeue(int V)
+    {
+    	V = a[rear];
+        rear = (rear + 1)%a.Length;
+        numberOfElements = numberOfElements - 1;
+    }
+
+}
+
+
+/*
+
+method Main() 
+{
+    var q:Queue := new Queue(4);
+    var r:int; 
+
+    q.Enqueue(1);
+    r := q.Dequeue();
+    q.Enqueue(2);
+    r := q.Dequeue();
+    q.Enqueue(3);
+    if (!q.Full())  
+    { q.Enqueue(4); }
+    r := q.Dequeue();
+    if (!q.Empty())
+    { r := q.Dequeue(); }
+    // q.Enqueue(5);
+    // q.Enqueue(5);
+    // q.Enqueue(5);
+    // q.Enqueue(5);
+    // q.Enqueue(5);
+}
+
+*/
