handout2.dfy
@@ -34,21 +34,29 @@ class PersonDB
         size := 0;
     }
 
+
+	//Deprecated
     method add() returns(pos:int)
     modifies this.people, this`size  // use ` to modify a variable, . for objects or collections
 	//requires this.people != null
 	//requires this.people != null
 	//ensures pos < this.people.Length
-    ensures size < this.people.Length	//people array cannot be full
+    ensures size <= this.people.Length	//people array cannot be full
     {
         if( 0 <= size < people.Length ) 
         {
             people[size] := new Row();
             size := size + 1;
         }
+		if( size >= people.Length)
+		{
+			size := people.Length;
+		}
         pos := size-1;
     }
 
+
+	//Deprecated
     method delete(i:int) 
     modifies this.people
     {
@@ -61,7 +69,7 @@ class PersonDB
     method find(i:int) returns (p:Person)
     requires 0 < i < size    
  	{
- 		p := null;
+ 		p := new Person(); //Returns an empty person because it can't be null
  		if( people[i] != null)
         {
 	 		if(people[i].name.Length > 0 && people[i].age >= 0)
@@ -81,13 +89,13 @@ class Person
 	var id:int;
  	var name:array<char>; 
 	var age:int;
-	var con:PersonDB;
+	var con:PersonDB?;
 
  	function Transient():bool
  	reads this
  	{ con == null && id == -1 }
  	
- 	function Persitent():bool
+ 	function Persistent():bool
  	reads this
  	{ id > -1 && con != null } 
 
@@ -101,31 +109,57 @@ class Person
 
  	method save(c:PersonDB)
  	modifies this
+	modifies c.people, c`size
  	requires this.name.Length > 0
  	requires this.age >= 0
-	requires c.people != null
- 	requires c.size < c.people.Length
- 	requires Transient() || Persitent()
- 	ensures Persitent()
+	//requires c.people != null
+ 	requires c.size <= c.people.Length
+ 	requires Transient() || Persistent()
+ 	ensures Persistent()
  	{	
- 		var pos := c.add();
+
+		var pos := -1;
+
+		if( 0 <= c.size < c.people.Length ) 
+        {
+            c.people[c.size] := new Row();
+			pos := c.size;
+            c.size := c.size + 1;
+        }
+		if( c.size >= c.people.Length)
+		{
+			c.size := c.people.Length;
+			c.people[c.size-1] := new Row();
+		}
+
  		c.people[pos].setName(this.name);
  		c.people[pos].setAge(this.age);
  		this.id := pos;
  		this.con := c;
  	}
 
- 	method delete()
+ 	method delete(c:PersonDB)
  	modifies this
- 	requires Persitent()
+	modifies c.people
+ 	requires Persistent()
  	ensures Transient()
  	{
- 		con.delete(this.id);
+ 		//con.delete(this.id);
+
+        if( 0 <= id < c.people.Length )
+        {
+            c.people[id] := null;
+        }
+
  		this.id := -1;
+		name := new char[0]; 
+		age := 0; 
+		this.con := null;
  	}
 
  	method close(c:PersonDB)
- 	requires Persitent()
+	modifies this
+ 	requires Persistent()
  	ensures Detatched()
  	{
  		this.con := null;
@@ -133,7 +167,8 @@ class Person
 
  	method update(c:PersonDB)
  	modifies this
- 	ensures Persitent()
+	requires Detatched()
+ 	ensures Persistent()
  	{
  		this.con := c;
  	}
@@ -171,7 +206,19 @@ class main
 {
 	method test()
 	{
+		//Creates a person and a database, stores it, closes, updates, closes again and deletes
 		var c:PersonDB := new PersonDB();
 		var p:Person := new Person();
+		var name := new char[10];
+		name[0] := 't';name[1] := 'e';name[2] := 's';name[3] := 't';name[4] := 'e';
+		p.setName(name);
+		p.setAge(22);
+		//var position := c.add();
+		p.save(c);
+		p.close(c);
+		p.update(c);
+		p.close(c);
+		p.delete(c);
+
 	}	
 }
