Aula4/42832_Luis_Correia_HO2.dfy
@@ -1,0 +1,224 @@
+class Row {
+	var name:array<char>;
+ 	var age:int; 
+
+	constructor ()
+ 	{ name := new char[0] ; age := 0; }
+
+
+ 	method setName(a:array<char>)
+ 	modifies this
+ 	requires a.Length > 0
+ 	ensures this.name.Length > 0
+ 	{
+ 		this.name := a;
+ 	}
+
+ 	method setAge(n:int)
+ 	modifies this
+ 	requires n >= 0;
+ 	ensures this.age >= 0;
+ 	{
+		this.age := n; 		
+ 	}
+}
+
+class PersonDB
+{
+	var people:array<Row?>;
+ 	var size:int; 
+
+    constructor() 
+    {
+        people := new Row?[10]; 
+        size := 0;
+    }
+
+
+	//Deprecated
+    method add() returns(pos:int)
+    modifies this.people, this`size  // use ` to modify a variable, . for objects or collections
+	//requires this.people != null
+	//requires this.people != null
+	//ensures pos < this.people.Length
+    ensures size <= this.people.Length	//people array cannot be full
+    {
+        if( 0 <= size < people.Length ) 
+        {
+            people[size] := new Row();
+            size := size + 1;
+        }
+		if( size >= people.Length)
+		{
+			size := people.Length;
+		}
+        pos := size-1;
+    }
+
+
+	//Deprecated
+    method delete(i:int) 
+    modifies this.people
+    {
+        if( 0 <= i < people.Length )
+        {
+            people[i] := null;
+        }
+    }
+
+    method find(i:int) returns (p:Person)
+    requires 0 < i < size    
+ 	{
+ 		p := new Person(); //Returns an empty person because it can't be null
+ 		if( people[i] != null)
+        {
+	 		if(people[i].name.Length > 0 && people[i].age >= 0)
+	 		{
+		 		p := new Person();
+		 		p.setAge(people[i].age);
+		 		p.setName(people[i].name);
+		 		p.setDB(this);
+	 		}
+        }
+ 	}
+}
+
+
+class Person
+{
+	var id:int;
+ 	var name:array<char>; 
+	var age:int;
+	var con:PersonDB?;
+
+ 	function Transient():bool
+ 	reads this
+ 	{ con == null && id == -1 }
+ 	
+ 	function Persistent():bool
+ 	reads this
+ 	{ id > -1 && con != null } 
+
+ 	function Detatched():bool
+ 	reads this
+ 	{ id > -1 && con == null} 
+
+	constructor ()
+ 	ensures Transient()
+ 	{ id := -1; name := new char[0]; age := 0; con := null; }
+
+ 	method save(c:PersonDB)
+ 	modifies this
+	modifies c.people, c`size
+ 	requires this.name.Length > 0
+ 	requires this.age >= 0
+	//requires c.people != null
+ 	requires c.size <= c.people.Length
+ 	requires Transient() || Persistent()
+ 	ensures Persistent()
+ 	{	
+
+		var pos := -1;
+
+		if( 0 <= c.size < c.people.Length ) 
+        {
+            c.people[c.size] := new Row();
+			pos := c.size;
+            c.size := c.size + 1;
+        }
+		if( c.size >= c.people.Length)
+		{
+			c.size := c.people.Length;
+			c.people[c.size-1] := new Row();
+		}
+
+ 		c.people[pos].setName(this.name);
+ 		c.people[pos].setAge(this.age);
+ 		this.id := pos;
+ 		this.con := c;
+ 	}
+
+ 	method delete(c:PersonDB)
+ 	modifies this
+	modifies c.people
+ 	requires Persistent()
+ 	ensures Transient()
+ 	{
+ 		//con.delete(this.id);
+
+        if( 0 <= id < c.people.Length )
+        {
+            c.people[id] := null;
+        }
+
+ 		this.id := -1;
+		name := new char[0]; 
+		age := 0; 
+		this.con := null;
+ 	}
+
+ 	method close(c:PersonDB)
+	modifies this
+ 	requires Persistent()
+ 	ensures Detatched()
+ 	{
+ 		this.con := null;
+ 	}
+
+ 	method update(c:PersonDB)
+ 	modifies this
+	requires Detatched()
+ 	ensures Persistent()
+ 	{
+ 		this.con := c;
+ 	}
+
+ 	method setName(a:array<char>)
+ 	modifies this
+ 	requires a.Length > 0
+ 	ensures this.name.Length > 0
+ 	{
+ 		this.name := a;
+ 	}
+
+ 	method setAge(n:int)
+ 	modifies this
+ 	requires n >= 0;
+ 	ensures this.age >= 0;
+ 	{
+		this.age := n; 		
+ 	}
+
+ 	method setID(i:int)
+ 	modifies this
+ 	{
+ 		this.id := i;
+ 	}
+
+ 	method setDB(db:PersonDB)
+ 	modifies this
+ 	{
+ 		this.con := db;
+ 	}
+}
+
+class main
+{
+	method test()
+	{
+		//Creates a person and a database, stores it, closes, updates, closes again and deletes
+		var c:PersonDB := new PersonDB();
+		var p:Person := new Person();
+		var name := new char[10];
+		name[0] := 't';name[1] := 'e';name[2] := 's';name[3] := 't';name[4] := 'e';
+		p.setName(name);
+		p.setAge(22);
+		//var position := c.add();
+		p.save(c);
+		p.close(c);
+		p.update(c);
+		p.close(c);
+		p.delete(c);
+
+	}	
+}
