Exercises/Test.dfy
@@ -1,0 +1,236 @@
+
+
+//method a(x:int) returns (y:int)
+//  requires -sqrt(2) <= x <= sqrt(2)
+//  ensures y <= 2
+//{
+//  y:=x*x;
+//}
+
+
+method mix(a:array<int>, b:array<int>, m:array<int>, n:int)
+modifies m
+requires 0 <= n <= a.Length
+requires 0 <= n <= b.Length
+requires 0 <= 2*n <= m.Length
+ensures forall i,k:int :: 0 <= k < 2*n && 0 <= i < n && k%2 == 0 ==> m[k] == a[i]
+ensures forall i,k:int :: 0 <= k < 2*n && 0 <= i < n && k%2 == 1 ==> m[k] == b[i]
+{
+    var i : int := 0;
+    var j : int := 0;
+    while(i < n)
+    decreases n - i
+    invariant 0 <= i <= n
+    invariant 0 <= j < 2*n
+    invariant forall l,k:int :: 0 <= k < j && 0 < l < i && k%2 == 0 ==> m[k] == a[l]
+    invariant forall l,k:int :: 0 <= k < j && 0 < l < i && k%2 == 1 ==> m[k] == b[l]
+
+    {
+        m[j] := a[i];
+        m[j+1] := b[i];
+        i := i+1;
+        j := j+2;
+    }
+}
+
+
+
+method mirror(a:array<int>, b:array<int>, n:int) returns (r:bool) 
+requires 0 <= n <= a.Length
+requires 0 <= n <= b.Length
+
+ensures   true ==> forall l : int :: 0 <= l < n ==> a[l] == b[n-1-l]
+ensures   false ==> exists l : int :: 0 <= l < n ==> a[l] != b[n-1-l]
+{ 
+   var i : int := 0; 
+   r := true; 
+
+   while(i<n)
+   decreases n-i 
+   invariant 0 <= i <= n
+   invariant r == true ==> forall l : int :: 0 <= l < i ==> a[l] == b[i-1-l]
+   invariant r ==  false ==> exists l : int :: 0 <= l < i ==> a[l] != b[i-1-l]
+   { 
+      if (a[i] != b[n-1-i]) 
+         {  
+           r := false; 
+          } 
+      i := i+1; 
+   } 
+}	
+
+
+
+method is_prime(n:int) returns (b:bool) 
+requires n >= 0
+ensures b <==> forall i::1<i<n ==> n % i != 0
+{ 
+   var d:int :=2; 
+   b := true;
+
+   if (n>1) 
+   { 
+
+   while(d<n && b)
+   decreases n-d
+   invariant d <= n
+   invariant b <==> forall l :: 1 < l < d ==> d*l != 0
+   { 
+      if ( n % d == 0) { b := false ; } 
+      d := d + 1; 
+   }  
+   } 
+} 
+
+
+
+method IndexOf(a:array<char>, n:int, K:char) returns (pos:int)
+requires 0 <= n <= a.Length
+ensures -1 <= pos < n
+ensures -1 < pos ==> a[pos] == K
+ensures pos == -1 ==> forall j:int :: 0 <= j < n ==> a[j] != K
+{
+    pos := -1;
+    var i:int := 0;
+
+    while(i < n)
+    decreases n - i
+    invariant 0 <= i <= n
+    invariant -1 <= pos < i
+    invariant -1 < pos ==> a[pos] == K
+    invariant pos == -1 ==> forall j:int :: 0 <= j < i ==> a[j] != K
+    {
+        if (a[i] == K)
+        {
+            pos := i;
+        }
+        i:= i+1;
+    }
+}
+
+
+
+method FillK(a:array<char>, n:int, K:char) returns (s:bool)
+requires 0 <= n <= a.Length
+ensures s <==> forall j:int :: 0 <= j < n ==> a[j] == K
+{
+    var i:int := 0;
+    s := true;
+    while(i < n && s == true)
+    decreases n - i
+    invariant 0 <= i <= n
+    invariant s <==> forall j:int :: 0 <= j < i ==> a[j] == K
+    {
+        if(a[i] != K)
+        {
+            s := false;
+        }
+        i := i + 1;
+    }
+}
+
+
+method FillKTF(a:array<char>, n:int, K:char) returns (s:bool)
+requires 0 <= n <= a.Length
+ensures s == true ==> forall j:int :: 0 <= j < n ==> a[j] == K
+ensures s == false ==> exists j:int :: 0 <= j < n && a[j] != K
+{
+    var i:int := 0;
+    s := true;
+    while(i < n && s == true)
+    decreases n - i
+    invariant 0 <= i <= n
+    invariant s == true ==> forall j:int :: 0 <= j < i ==> a[j] == K
+    invariant s == false ==> exists j:int :: 0 <= j < i && a[j] != K
+    {
+        if(a[i] != K)
+        {
+            s := false;
+        }
+        i := i + 1;
+    }
+}
+
+
+method FillKExists(a:array<char>, n:int, K:char) returns (s:bool)
+requires 0 <= n <= a.Length
+ensures !s <==> exists j:int :: 0 <= j < n && a[j] != K
+{
+    var i:int := 0;
+    s := true;
+    while(i < n && s == true)
+    decreases n - i
+    invariant 0 <= i <= n
+    invariant !s <==> exists j:int :: 0 <= j < i && a[j] != K
+    {
+        if(a[i] != K)
+        {
+            s := false;
+        }
+        i := i + 1;
+    }
+}
+
+
+method Reverse(a:array<int>, n:int) returns (b:array<int>)
+requires 0 <= n <= a.Length
+ensures a.Length == b.Length
+ensures forall j:int :: 0 <= j < n ==> a[j] == b[n-j-1]
+ensures forall k:int :: n <= k < a.Length ==> a[k] == b[k]
+{
+    b:= new int[a.Length];
+    
+    var i := 0;
+    while(i<n)
+    decreases n-i
+    invariant 0 <= i <= n
+    invariant forall j:int :: 0 <= j < i ==> a[j] == b[n-j-1]
+    {
+        b[n-i-1] := a[i];
+        i := i + 1;
+    }
+
+    while(i < a.Length)
+    decreases a.Length - i
+    invariant n <= i <= a.Length
+    invariant forall j:int :: 0 <= j < n ==> a[j] == b[n-j-1]
+    invariant forall k:int :: n <= k < i ==> a[k] == b[k]
+    {
+        b[i] := a[i];
+        i := i + 1;
+    }
+
+} 
+
+
+function Abs(x: int):int 
+    //ensures (x < 0 && y == -x) || (x >= 0 && y == x)
+{
+    if x < 0 then
+    -x
+    else
+    x
+
+}
+
+method func(x:int, y:int) returns (z:int)
+requires Abs(x-y) <= 2
+ensures 0 <= z <=2 
+//ensures z >= 0 ==> x > y
+//ensures x-y <= 2
+//ensures y-x <= 2
+//ensures x > y ==> z == y-x
+//ensures y > x ==> z == x-y
+//ensures Abs(z) <= 2
+//ensures z != 3
+{
+    if(x>y)
+    {z:=x-y;}
+    else
+    {z:=y-x;}
+}
+
+
+method Main() {
+  print "hello, Dafny\n";
+}
